\documentclass{article}

\usepackage{amsmath}

\usepackage{amssymb}

\usepackage{amsthm}

\usepackage{graphicx}



\newtheorem{definition}{Definition}

\newtheorem{property}{Property}

\newtheorem{ex}{Example}

\newtheorem{thm}{Theorem}

\newtheorem{lemma}{Lemma}

\newtheorem{prop}{Proposition}



\begin{document}
\begin{definition}
	The derivative of a function $f(x)$ is noted as $f'(x)$. It is the same as computing the instantaneous rate of change at point x.
\end{definition}

\begin{thm}
We have a table of rules of taking derivatives.
	
\begin{center}
	\includegraphics*[width=12cm]{deriv11.png}
\end{center}
\end{thm}

\begin{ex}
	Find the derivative of the function $f(x) = \sqrt{x^3}$ at point $x=4$.
	
	\begin{proof}
		From the table, we see that 
		\[ f'(x) = (x^{\frac{3}{2}})' = \frac{3}{2} x^{\frac{1}{2}} \]
		Thus, $f'(4) = \frac{3}{2}4^{\frac{1}{2}} = 3$
	\end{proof}
\end{ex}

In order to compute the derivative of more complicated functions, we need the following properties.
\begin{property}
	\begin{align}
	&(f\pm g)' = f' \pm g'\\
	&(cf)' = cf'\\
	&(fg)' = f'g+fg'\\
	&(\frac{f}{g})' = \frac{f'g-fg'}{g^2}\\
	& f(g)' = f'(g)g'
	\end{align}
\end{property}


\begin{ex}
	Find the derivative of the function $f(x)= x^2 + \cos x$.
	\begin{proof}
		\[ f'(x) = (x^2)' + (2\cos x)' = 2x - 2\sin x \]
	\end{proof}
\end{ex}

\begin{ex}
	Find the derivative of the function $f(x) = x\sin x$.
	
	\begin{proof}
		\[ f'(x) = (x)'\sin x + x(\sin x)' = \sin x + x\cos x \]
	\end{proof}
\end{ex}

\begin{ex}
	Find the slope of the tangent line of the function 
	\[ f(x) = \frac{x^2}{x+1} \]
	at point $x=1$.
	
	\begin{proof}
		\begin{align*}
		f'(x) &= \left(\frac{x^2}{x+1}\right)'\\
		&= \frac{(x^2)'(x+1)-(x^2)(x+1)'}{(x+1)^2}\\
		&= \frac{2x(x+1)-x^2}{(x+1)^2}\\
		&= \frac{x^2 - 2x}{(x+1)^2}
		\end{align*}
		
		Thus the slope of $f(x)$ at $x=1$
		\[ f'(1) = \frac{1^2 -2\times1}{(1+1)^2} = -\frac{1}{4} \]
	\end{proof}	
\end{ex}


\begin{ex}
	Find the derivative of the composite function $f(x) = (x^2+2x)^4$.
	\begin{proof}
		Let $g(x) = x^4$ and $h(x)= x^2+2x$. Then $f(x) = g(h(x))$. Thus
		\[ f'(x) = g'(h(x))h'(x) = 4(x^2+2x)^3(2x+2)  \]
	\end{proof}
\end{ex}



\end{document}

